src/goose_lang/logical_reln_fund.v
@@ -541,7 +541,8 @@ Proof.
     iDestruct (heap_mapsto_na_acc with "Hpts'") as "(Hpts'&_)".
     rewrite ?na_heap_mapsto_eq /na_heap_mapsto_def.
     iDestruct (na_heap_mapsto_st_frac_valid2 with "Hpts Hpts'") as %Hval.
-    apply Z2Qc_inj_le in Hval. lia.
+    apply Qp_to_Qc_inj_le in Hval; cbv in Hval.
+    contradiction.
   }
   {
     iDestruct "Hreaders" as (q q' n') "(>%&>Hfc&>Hspts'&Hspts'_clo&>Hpts'&_)".
